WIP

Functional Algorithms/Sort.v
@@ -1,10 +1,65 @@
+Require Import PeanoNat.
+Require Import Permutation.
 Require Import List.
+Import ListNotations.
 (* Require Import Perm. *)
 (* insert i l inserts i into its sorted place in list l.
    Precondition: l is sorted. *)
 
-Fixpoint insert (i : nat) (l : list nat) :=
+Fixpoint insert (i : nat) (l : list nat) : list nat :=
   match l with
   | [] => [i]
   | h :: t => if i <=? h then i :: h :: t else h :: insert i t
   end.
+
+Fixpoint sort (l : list nat) : list nat :=
+  match l with
+  | [] => []
+  | h :: t => insert h (sort t)
+  end.
+  
+Example sort_pi :
+  sort [3;1;4;1;5;9;2;6;5;3;5]
+  = [1;1;2;3;3;4;5;5;5;6;9].
+Proof.
+  simpl. reflexivity.
+Qed.
+  
+Compute insert 7 [1;3;4;8;12;14;18].
+
+Inductive sorted : list nat -> Prop :=
+| sorted_nil : sorted []
+| sorted_1 : forall x, sorted [x]
+| sorted_cons : forall x y l,
+    x <= y -> sorted (y :: l) -> sorted (x :: y :: l).
+
+
+Definition sorted'' (al : list nat) := forall i j,
+  i < j < length al ->
+  nth i al 0 <= nth j al 0.
+
+Definition sorted' (al : list nat) := forall i j iv jv,
+  i < j ->
+  nth_error al i = Some iv ->
+  nth_error al j = Some jv ->
+  iv <= jv.
+  
+Definition is_a_sorting_algorithm (f : list nat -> list nat) := forall al,
+  Permutation al (f al) /\ sorted (f al).
+
+Theorem insert_sorted:
+  forall a l, sorted l -> sorted( insert a l).
+Proof.
+  intros a l S. induction S. simpl.
+Qed.
+  
+  
+  
+  
+  
+  
+  
+  
+  
+  
+  
